examples/sys_regs.v
@@ -18,3 +18,54 @@ Definition sys_regs : list (reg_col_entry * valu) := [
   (RegColStruct "PSTATE" "nRW" , Val_Bits [BV{1} 0] );
   (RegColStruct "PSTATE" "D" , Val_Bits [BV{1} 1])
 ].
+
+Definition sys_regs_map : reg_map :=
+  <[ "SCTLR_EL2" := Val_Bits [BV{64} 0x0000000004000002] ]> $
+  <[ "SCR_EL3" := Val_Bits [BV{32} 0] ]> $
+  <[ "TCR_EL2" := Val_Bits [BV{64} 0] ]> $
+  <[ "CFG_ID_AA64PFR0_EL1_EL0" := Val_Bits [BV{4} 1] ]> $
+  <[ "CFG_ID_AA64PFR0_EL1_EL1" := Val_Bits [BV{4} 1] ]> $
+  <[ "CFG_ID_AA64PFR0_EL1_EL2" := Val_Bits [BV{4} 1] ]> $
+  <[ "CFG_ID_AA64PFR0_EL1_EL3" := Val_Bits [BV{4} 1] ]> $
+  <[ "OSLSR_EL1" := Val_Bits [BV{32} 0] ]> $
+  <[ "OSDLR_EL1" := Val_Bits [BV{32} 0] ]> $
+  <[ "EDSCR" := Val_Bits [BV{32} 0] ]> $
+  <[ "MPIDR_EL1" := Val_Bits [BV{64} 0] ]> $
+  <[ "PSTATE" := (Val_Struct
+    [("GE", Val_Poison); ("F", Val_Poison);
+    ("UAO", Val_Poison); ("C", Val_Bits [BV{1} 0]);
+    ("SP", Val_Bits [BV{1} 1]); ("N", Val_Bits [BV{1} 0]);
+    ("Q", Val_Poison); ("A", Val_Poison); ("SS", Val_Poison);
+    ("E", Val_Poison); ("TCO", Val_Poison); ("I", Val_Poison);
+    ("PAN", Val_Poison); ("M", Val_Poison); ("D", Val_Bits [BV{1} 1]);
+    ("nRW", Val_Bits [BV{1} 0]); ("EL", Val_Bits [BV{2} 2]);
+    ("IT", Val_Poison); ("IL", Val_Poison);
+    ("Z", Val_Bits [BV{1} 0]); ("BTYPE", Val_Poison);
+    ("SSBS", Val_Poison); ("T", Val_Poison); ("J", Val_Poison);
+    ("V", Val_Bits [BV{1} 0]); ("DIT", Val_Poison)]) ]> $ ∅.
+
+Section sys_regs.
+  Context `{!islaG Σ} `{!threadG}.
+
+  Lemma sys_regs_init regs:
+    regs_ctx regs -∗
+    ([∗ map] k↦y ∈ sys_regs_map, k ↦ᵣ y) ==∗
+    regs_ctx regs ∗
+    reg_col sys_regs ∗
+    "PSTATE" # "C" ↦ᵣ Val_Bits [BV{1} 0] ∗
+    "PSTATE" # "N" ↦ᵣ Val_Bits [BV{1} 0] ∗
+    "PSTATE" # "V" ↦ᵣ Val_Bits [BV{1} 0] ∗
+    "PSTATE" # "Z" ↦ᵣ Val_Bits [BV{1} 0].
+  Proof.
+    rewrite /reg_col/=.
+    repeat (rewrite big_sepM_insert;[ | by vm_compute]).
+    iIntros "Hctx H". repeat iDestruct "H" as "[$ H]".
+    iDestruct "H" as "[HPSTATE _]".
+    iMod (reg_mapsto_to_struct_reg_mapsto with "Hctx HPSTATE") as "[$ H]".
+    { simpl. repeat (constructor; [set_solver|]). constructor. }
+    simpl. repeat (iDestruct "H" as "[Hf H]"; first [ iFrame "Hf" | iClear "Hf"]).
+    done.
+  Qed.
+End sys_regs.
+
+Global Opaque sys_regs_map.
