examples/example.v
@@ -2,43 +2,8 @@ Require Import isla.base.
 Require Import isla.opsem.
 Require Import isla.automation.
 Require Import isla.adequacy.
-From isla.instructions Require Import load.
-
-
-(* Ltac solve_trace_step := by econstructor. *)
-(* Ltac do_trace_step := *)
-(*   apply: TraceStep'; [solve_trace_step | done |]; simpl. *)
-
-
-(* trace of add x1, x2, x3:
-  (declare-const v3359 (_ BitVec 64))
-  (declare-const v3361 (_ BitVec 64))
-  (read-reg |R2| nil v3359)
-  (define-const v3425 v3359)
-  (read-reg |R3| nil v3361)
-  (define-const v3426 v3361)
-  (define-const v3431 ((_ zero_extend 64) v3425))
-  (define-const v3432 ((_ zero_extend 64) v3426))
-  (define-const v3433 (bvadd v3431 v3432))
-  (define-const v3437 ((_ extract 63 0) v3433))
-  (define-const v3452 v3437)
-  (write-reg |R1| nil v3452)
-*)
-Definition trc_add_x1_x2_x3 : trc :=
-  [
-  Smt (DeclareConst 3359 (Ty_BitVec 64)) Mk_annot;
-  Smt (DeclareConst 3361 (Ty_BitVec 64)) Mk_annot;
-  ReadReg "R2" [] (Val_Symbolic 3359) Mk_annot;
-  Smt (DefineConst 3425 (Val (Val_Symbolic 3359) Mk_annot)) Mk_annot;
-  ReadReg "R3" [] (Val_Symbolic 3361) Mk_annot;
-  Smt (DefineConst 3426 (Val (Val_Symbolic 3361) Mk_annot)) Mk_annot;
-  Smt (DefineConst 3431 (Unop (ZeroExtend 64) (Val (Val_Symbolic 3425) Mk_annot) Mk_annot)) Mk_annot;
-  Smt (DefineConst 3432 (Unop (ZeroExtend 64) (Val (Val_Symbolic 3426) Mk_annot) Mk_annot)) Mk_annot;
-  Smt (DefineConst 3433 (Manyop (Bvmanyarith Bvadd) [Val (Val_Symbolic 3431) Mk_annot; Val (Val_Symbolic 3432) Mk_annot] Mk_annot)) Mk_annot;
-  Smt (DefineConst 3437 (Unop (Extract 63 0) (Val (Val_Symbolic 3433) Mk_annot) Mk_annot)) Mk_annot;
-  Smt (DefineConst 3452 (Val (Val_Symbolic 3437) Mk_annot)) Mk_annot;
-  WriteReg "R1" [] (Val_Symbolic 3452) Mk_annot
-].
+Require Import isla.examples.sys_regs.
+From isla.instructions Require Import bl_0x100 mov_w0_0 ret mov_x28_x0 mov_x0_1 b_0x8 cmp_x1_0.
 
 (*
 C:
@@ -48,83 +13,7 @@ int test() {
 compiled via GCC:
         mov     w0, 0
         ret
-
-trace of mov w0, 0:
-  (write-reg |R0| nil #x0000000000000000))
-
-trace of ret:
-(trace
-  (declare-const v3428 (_ BitVec 64))
-  (define-const v3429 v3428)
-  (read-reg |R30| nil v3429)
-  (define-const v3435 v3429)
-#  (write-reg |BTypeNext| nil #b00)
-  (define-const v3436 v3435)
-  (branch-address v3436)
-  (define-const v3437 v3435)
-# There are two generated traces, but they seem to do the same
-#  (define-const v3471 (= (bvor #b0 ((_ extract 0 0) (bvlshr v3437 #x0000000000000037))) #b1))
-#  (branch 0 "model/aarch_mem.sail 6170:20 - 6170:81")
-#  (assert v3471)
-  (write-reg |_PC| nil v3437)
-  (write-reg |__PC_changed| nil true))
-*)
-
-Definition trc_mov_w0_0 : trc := [
-   WriteReg "R0" [] (Val_Bits [BV{64} 0x0000000000000000]) Mk_annot
-  ].
-
-Definition trc_mov_x0_1 : trc := [
-   WriteReg "R0" [] (Val_Bits [BV{64} 0x0000000000000001]) Mk_annot
-  ].
-
-Definition trc_ret : trc := [
-  Smt (DeclareConst 3428 (Ty_BitVec 64)) Mk_annot;
-  Smt (DefineConst 3429 (Val (Val_Symbolic 3428) Mk_annot)) Mk_annot;
-  ReadReg "R30" nil (Val_Symbolic 3429) Mk_annot;
-  Smt (DefineConst 3435 (Val (Val_Symbolic 3429) Mk_annot)) Mk_annot;
-  (* WriteReg "BTypeNext" nil (Val_Bits 0) Mk_annot; *)
-  Smt (DefineConst 3436 (Val (Val_Symbolic 3435) Mk_annot)) Mk_annot;
-  BranchAddress (Val_Symbolic 3436) Mk_annot;
-  Smt (DefineConst 3437 (Val (Val_Symbolic 3435) Mk_annot)) Mk_annot;
-  WriteReg "_PC" nil (Val_Symbolic 3437) Mk_annot;
-  WriteReg "__PC_changed" nil (Val_Bool true) Mk_annot
-].
-
-(* trace of bl 0x100: (at address 0x0000000010300000)
-(trace
-  (read-reg |_PC| nil #x0000000010300000)
-  (write-reg |R30| nil #x0000000010300004)
-  (read-reg |_PC| nil #x0000000010300000)
-  (branch-address #x0000000010300100)
-  (write-reg |_PC| nil #x0000000010300100)
-  (write-reg |__PC_changed| nil true))
-*)
-Definition trc_bl_0x100 : trc := [
-  ReadReg "_PC" nil (Val_Bits [BV{64} 0x0000000010300000]) Mk_annot;
-  WriteReg "R30" nil (Val_Bits [BV{64} 0x0000000010300004]) Mk_annot;
-  ReadReg "_PC" nil (Val_Bits [BV{64} 0x0000000010300000]) Mk_annot;
-  BranchAddress (Val_Bits [BV{64} 0x0000000010300100]) Mk_annot;
-  WriteReg "_PC" nil (Val_Bits [BV{64} 0x0000000010300100]) Mk_annot;
-  WriteReg "__PC_changed" nil (Val_Bool true) Mk_annot
-].
-
-(* trace of mov x28, x0:
-trace
-  (declare-const v3368 (_ BitVec 64))
-  (define-const v3369 v3368)
-  (read-reg |R0| nil v3369)
-  (define-const v3450 (bvor #x0000000000000000 v3369))
-  (write-reg |R28| nil v3450))
-*)
-Definition trc_mov_OUT_x0 : trc := [
-  Smt (DeclareConst 3368 (Ty_BitVec 64)) Mk_annot;
-  Smt (DefineConst 3369 (Val (Val_Symbolic 3368) Mk_annot)) Mk_annot;
-  ReadReg "R0" nil (Val_Symbolic 3369) Mk_annot;
-  Smt (DefineConst 3450 (Manyop (Bvmanyarith Bvor) [Val (Val_Bits [BV{64} 0x0000000000000000]) Mk_annot; Val (Val_Symbolic 3369) Mk_annot] Mk_annot)) Mk_annot;
-  WriteReg "OUT" nil (Val_Symbolic 3450) Mk_annot
-].
-
+ *)
 
 Definition start_address := [BV{64} (0x0000000010300000 - 0x4)].
 Definition test_state_local := {|
@@ -135,17 +24,17 @@ Definition test_state_local := {|
     <[ "R30" := Val_Poison ]> $
     <[ "R1" := Val_Poison ]> $
     <[ "R0" := Val_Poison ]> $
-    <[ "OUT" := Val_Poison ]> $
-     ∅;
+    <[ "R28" := Val_Poison ]> $
+     sys_regs_map;
   seq_nb_state  := false;
 |}.
 
 Definition test_state_global := {|
     seq_instrs :=
-    <[ [BV{64} 0x0000000010300000] := [trc_bl_0x100]]> $   (* bl 0x100: (at address 0x0000000010300000 *)
-    <[ [BV{64} 0x0000000010300004] := [trc_mov_OUT_x0]]> $ (* mov OUT, x0 *)
-    <[ [BV{64} 0x0000000010300100] := [trc_mov_w0_0]]> $   (* mov w0, 0 *)
-    <[ [BV{64} 0x0000000010300104] := [trc_ret]]> $        (* ret *)
+    <[ [BV{64} 0x0000000010300000] := [bl_0x100_trace]]> $   (* bl 0x100 *)
+    <[ [BV{64} 0x0000000010300004] := [mov_x28_x0_trace]]> $ (* mov OUT, x0 *)
+    <[ [BV{64} 0x0000000010300100] := [mov_w0_0_trace]]> $   (* mov w0, 0 *)
+    <[ [BV{64} 0x0000000010300104] := [ret_trace]]> $        (* ret *)
     ∅;
     seq_mem := ∅
 |}.
@@ -154,17 +43,18 @@ Definition test_state_global := {|
 Definition test_state_spec : list seq_label := [ SInstrTrap ([BV{64} 0x0000000010300008]) ].
 
 Lemma test_state_iris `{!islaG Σ} `{!threadG} :
-  instr 0x0000000010300000 (Some [trc_bl_0x100]) -∗
-  instr 0x0000000010300004 (Some [trc_mov_OUT_x0]) -∗
+  instr 0x0000000010300000 (Some [bl_0x100_trace]) -∗
+  instr 0x0000000010300004 (Some [mov_x28_x0_trace]) -∗
   instr 0x0000000010300008 None -∗
-  instr 0x0000000010300100 (Some [trc_mov_w0_0]) -∗
-  instr 0x0000000010300104 (Some [trc_ret]) -∗
+  instr 0x0000000010300100 (Some [mov_w0_0_trace]) -∗
+  instr 0x0000000010300104 (Some [ret_trace]) -∗
+  reg_col sys_regs -∗
   "_PC" ↦ᵣ Val_Bits start_address -∗
   "__PC_changed" ↦ᵣ Val_Bool false -∗
   "R30" ↦ᵣ Val_Poison -∗
   "R1" ↦ᵣ Val_Poison -∗
   "R0" ↦ᵣ Val_Poison -∗
-  "OUT" ↦ᵣ Val_Poison -∗
+  "R28" ↦ᵣ Val_Poison -∗
   spec_trace test_state_spec -∗
   WPasm [].
 Proof.
@@ -181,53 +71,54 @@ Proof.
   set Σ : gFunctors := #[islaΣ].
   apply: (isla_adequacy Σ) => //.
   iIntros (?) "#Hi Hspec /= !>". iSplitL => //.
-  iIntros (?) "/=".
-  do 6 rewrite big_sepM_insert //=.
-  iIntros "(?&?&?&?&?&?&?)".
-  iApply (test_state_iris with "[] [] [] [] [] [$] [$] [$] [$] [$] [$] [$]").
+  iIntros (?).
+  do 6 (rewrite big_sepM_insert; [|by vm_compute]).
+  iIntros "(?&?&?&?&?&?&Hregs)".
+  iApply wp_asm_thread_ctx. iIntros (?) "Hctx".
+  iMod (sys_regs_init with "Hctx Hregs") as "(?&?&?)". iModIntro. iFrame.
+  iApply (test_state_iris with "[] [] [] [] [] [$] [$] [$] [$] [$] [$] [$] [$]").
   all: try by unshelve iApply (instr_intro with "Hi").
 Qed.
 
 Definition test_state_fn1_spec `{!islaG Σ} `{!threadG} : iProp Σ :=
   ∃ (r : addr) v0,
+    reg_col sys_regs ∗
     "R0" ↦ᵣ v0 ∗
     "R30" ↦ᵣ Val_Bits r ∗
     instr_pre (bv_unsigned r) (
+      reg_col sys_regs ∗
       "R30" ↦ᵣ Val_Bits r ∗
       "R0" ↦ᵣ Val_Bits [BV{64} 0] ∗ True
     ).
 Arguments test_state_fn1_spec /.
 
 Lemma test_state_iris_fn1 `{!islaG Σ} `{!threadG} :
-  instr 0x0000000010300100 (Some [trc_mov_w0_0]) -∗
-  instr 0x0000000010300104 (Some [trc_ret]) -∗
+  instr 0x0000000010300100 (Some [mov_w0_0_trace]) -∗
+  instr 0x0000000010300104 (Some [ret_trace]) -∗
   instr_body 0x0000000010300100 test_state_fn1_spec.
 Proof.
   iStartProof.
   repeat liAStep; liShow.
-  Unshelve.
-  all: done.
 Qed.
 
 Definition test_state_fn2_spec `{!islaG Σ} `{!threadG} : iProp Σ :=
+  reg_col sys_regs ∗
   "R30" ↦ᵣ Val_Poison ∗
   "R1" ↦ᵣ Val_Poison ∗
   "R0" ↦ᵣ Val_Poison ∗
-  "OUT" ↦ᵣ Val_Poison ∗
+  "R28" ↦ᵣ Val_Poison ∗
   spec_trace test_state_spec.
 Arguments test_state_fn2_spec /.
 
 Lemma test_state_iris_fn2 `{!islaG Σ} `{!threadG} :
-  instr 0x0000000010300000 (Some [trc_bl_0x100]) -∗
-  instr 0x0000000010300004 (Some [trc_mov_OUT_x0]) -∗
+  instr 0x0000000010300000 (Some [bl_0x100_trace]) -∗
+  instr 0x0000000010300004 (Some [mov_x28_x0_trace]) -∗
   instr 0x0000000010300008 None -∗
   □ instr_pre 0x0000000010300100 test_state_fn1_spec -∗
   instr_body 0x0000000010300000 test_state_fn2_spec.
 Proof.
   iStartProof.
   repeat liAStep; liShow.
-  Unshelve.
-  all: done.
 Qed.
 
 Lemma test_state_adequate' κs t2 σ2 n:
@@ -240,8 +131,10 @@ Proof.
   apply: (isla_adequacy Σ) => //.
   iIntros (?) "#Hi Hspec /= !>". iSplitL => //.
   iIntros (?) "/=".
-  do 6 rewrite big_sepM_insert //=.
-  iIntros "(HPC&Hchanged&?&?&?&?&?)".
+  do 6 (rewrite big_sepM_insert; [|by vm_compute]).
+  iIntros "(HPC&Hchanged&?&?&?&?&Hregs)".
+  iApply wp_asm_thread_ctx. iIntros (?) "Hctx".
+  iMod (sys_regs_init with "Hctx Hregs") as "(?&?&?)". iModIntro. iFrame.
 
   iAssert (
       □ instr_body 0x0000000010300000 test_state_fn2_spec ∗
@@ -260,86 +153,6 @@ Proof.
   - iExists _, _, _. by iFrame.
   - iFrame.
 Qed.
-
-
-(* trace of cmp x1, 0:
-  (declare-const v3370 (_ BitVec 64))
-  (define-const v3371 v3370)
-  (read-reg |R1| nil v3371)
-  (define-const v3435 v3371)
-  (define-const v3440 (bvadd (bvadd ((_ zero_extend 64) v3435) #x0000000000000000ffffffffffffffff) #x00000000000000000000000000000001))
-  (define-const v3444 ((_ extract 63 0) v3440))
-  (define-const v3457 (concat (concat (concat (bvor (bvand #b0 (bvnot #b1)) ((_ extract 0 0) (bvlshr v3444 ((_ extract 63 0) #x0000000000000000000000000000003f)))) (ite (= v3444 #x0000000000000000) #b1 #b0)) (ite (= ((_ zero_extend 64) v3444) v3440) #b0 #b1)) (ite (= ((_ sign_extend 64) v3444) (bvadd (bvadd ((_ sign_extend 64) v3435) #xffffffffffffffffffffffffffffffff) #x00000000000000000000000000000001)) #b0 #b1)))
-  (define-const v3459 ((_ extract 3 3) v3457))
-  (read-reg |PSTATE| ((_ field |N|)) (_ struct (|GE| v27) (|F| #b1) (|UAO| v23) (|C| v20) (|SP| #b1) (|N| v29) (|Q| v21) (|A| #b1) (|SS| #b0) (|E| v33) (|TCO| v13) (|I| #b1) (|PAN| v35) (|M| v12) (|D| #b1) (|nRW| #b0) (|EL| #b00) (|IT| v31) (|IL| #b0) (|Z| v15) (|BTYPE| v19) (|SSBS| v28) (|T| v16) (|J| v32) (|V| v25) (|DIT| #b0)))
-  (write-reg |PSTATE| ((_ field |N|)) (_ struct (|GE| v27) (|F| #b1) (|UAO| v23) (|C| v20) (|SP| #b1) (|N| v3459) (|Q| v21) (|A| #b1) (|SS| #b0) (|E| v33) (|TCO| v13) (|I| #b1) (|PAN| v35) (|M| v12) (|D| #b1) (|nRW| #b0) (|EL| #b00) (|IT| v31) (|IL| #b0) (|Z| v15) (|BTYPE| v19) (|SSBS| v28) (|T| v16) (|J| v32) (|V| v25) (|DIT| #b0)))
-  (define-const v3460 ((_ extract 2 2) v3457))
-  (read-reg |PSTATE| ((_ field |Z|)) (_ struct (|GE| v27) (|F| #b1) (|UAO| v23) (|C| v20) (|SP| #b1) (|N| v3459) (|Q| v21) (|A| #b1) (|SS| #b0) (|E| v33) (|TCO| v13) (|I| #b1) (|PAN| v35) (|M| v12) (|D| #b1) (|nRW| #b0) (|EL| #b00) (|IT| v31) (|IL| #b0) (|Z| v15) (|BTYPE| v19) (|SSBS| v28) (|T| v16) (|J| v32) (|V| v25) (|DIT| #b0)))
-  (write-reg |PSTATE| ((_ field |Z|)) (_ struct (|GE| v27) (|F| #b1) (|UAO| v23) (|C| v20) (|SP| #b1) (|N| v3459) (|Q| v21) (|A| #b1) (|SS| #b0) (|E| v33) (|TCO| v13) (|I| #b1) (|PAN| v35) (|M| v12) (|D| #b1) (|nRW| #b0) (|EL| #b00) (|IT| v31) (|IL| #b0) (|Z| v3460) (|BTYPE| v19) (|SSBS| v28) (|T| v16) (|J| v32) (|V| v25) (|DIT| #b0)))
-  (define-const v3461 ((_ extract 1 1) v3457))
-  (read-reg |PSTATE| ((_ field |C|)) (_ struct (|GE| v27) (|F| #b1) (|UAO| v23) (|C| v20) (|SP| #b1) (|N| v3459) (|Q| v21) (|A| #b1) (|SS| #b0) (|E| v33) (|TCO| v13) (|I| #b1) (|PAN| v35) (|M| v12) (|D| #b1) (|nRW| #b0) (|EL| #b00) (|IT| v31) (|IL| #b0) (|Z| v3460) (|BTYPE| v19) (|SSBS| v28) (|T| v16) (|J| v32) (|V| v25) (|DIT| #b0)))
-  (write-reg |PSTATE| ((_ field |C|)) (_ struct (|GE| v27) (|F| #b1) (|UAO| v23) (|C| v3461) (|SP| #b1) (|N| v3459) (|Q| v21) (|A| #b1) (|SS| #b0) (|E| v33) (|TCO| v13) (|I| #b1) (|PAN| v35) (|M| v12) (|D| #b1) (|nRW| #b0) (|EL| #b00) (|IT| v31) (|IL| #b0) (|Z| v3460) (|BTYPE| v19) (|SSBS| v28) (|T| v16) (|J| v32) (|V| v25) (|DIT| #b0)))
-  (define-const v3462 ((_ extract 0 0) v3457))
-  (read-reg |PSTATE| ((_ field |V|)) (_ struct (|GE| v27) (|F| #b1) (|UAO| v23) (|C| v3461) (|SP| #b1) (|N| v3459) (|Q| v21) (|A| #b1) (|SS| #b0) (|E| v33) (|TCO| v13) (|I| #b1) (|PAN| v35) (|M| v12) (|D| #b1) (|nRW| #b0) (|EL| #b00) (|IT| v31) (|IL| #b0) (|Z| v3460) (|BTYPE| v19) (|SSBS| v28) (|T| v16) (|J| v32) (|V| v25) (|DIT| #b0)))
-  (write-reg |PSTATE| ((_ field |V|)) (_ struct (|GE| v27) (|F| #b1) (|UAO| v23) (|C| v3461) (|SP| #b1) (|N| v3459) (|Q| v21) (|A| #b1) (|SS| #b0) (|E| v33) (|TCO| v13) (|I| #b1) (|PAN| v35) (|M| v12) (|D| #b1) (|nRW| #b0) (|EL| #b00) (|IT| v31) (|IL| #b0) (|Z| v3460) (|BTYPE| v19) (|SSBS| v28) (|T| v16) (|J| v32) (|V| v3462) (|DIT| #b0))))
-*)
-Definition trc_cmp_x1_0 : trc := [
-  Smt (DeclareConst 15 (Ty_BitVec 1)) Mk_annot;
-  Smt (DeclareConst 20 (Ty_BitVec 1)) Mk_annot;
-  Smt (DeclareConst 25 (Ty_BitVec 1)) Mk_annot;
-  Smt (DeclareConst 29 (Ty_BitVec 1)) Mk_annot;
-  Smt (DeclareConst 3370 (Ty_BitVec 64)) Mk_annot;
-  Smt (DefineConst 3371 (Val (Val_Symbolic 3370) Mk_annot)) Mk_annot;
-  ReadReg "R1" nil (Val_Symbolic 3371) Mk_annot;
-  Smt (DefineConst 3435 (Val (Val_Symbolic 3371) Mk_annot)) Mk_annot;
-  Smt (DefineConst 3440 (Manyop (Bvmanyarith Bvadd) [
-    Manyop (Bvmanyarith Bvadd) [
-      (Unop (ZeroExtend 64) (Val (Val_Symbolic 3435) Mk_annot) Mk_annot);
-      (Val (Val_Bits [BV{128} 0x0000000000000000ffffffffffffffff]) Mk_annot)
-      ] Mk_annot;
-    (Val (Val_Bits [BV{128} 0x00000000000000000000000000000001]) Mk_annot)
-  ] Mk_annot)) Mk_annot;
-  Smt (DefineConst 3444 (Unop (Extract 63 0) (Val (Val_Symbolic 3440) Mk_annot) Mk_annot)) Mk_annot;
-  Smt (DefineConst 3457 (Manyop Concat [
-    Manyop Concat [
-      Manyop Concat [
-        Manyop (Bvmanyarith Bvor) [
-          Manyop (Bvmanyarith Bvand) [
-            Val (Val_Bits [BV{1} 0]) Mk_annot;
-            Unop Bvnot (Val (Val_Bits [BV{1} 1]) Mk_annot) Mk_annot
-          ] Mk_annot;
-            (Unop (Extract 0 0) (Binop (Bvarith Bvlshr)
-               (Val (Val_Symbolic 3444) Mk_annot)
-               (Unop (Extract 63 0) (Val (Val_Bits [BV{128} 0x0000000000000000000000000000003f]) Mk_annot) Mk_annot) Mk_annot) Mk_annot)
-        ] Mk_annot;
-        Ite (Binop Eq (Val (Val_Symbolic 3444) Mk_annot) (Val (Val_Bits [BV{64} 0x0000000000000000]) Mk_annot) Mk_annot) (Val (Val_Bits [BV{1} 1]) Mk_annot) (Val (Val_Bits [BV{1} 0]) Mk_annot) Mk_annot
-       ] Mk_annot;
-        Ite (Binop Eq (Unop (ZeroExtend 64) (Val (Val_Symbolic 3444) Mk_annot) Mk_annot) (Val (Val_Symbolic 3440) Mk_annot) Mk_annot) (Val (Val_Bits [BV{1} 0]) Mk_annot) (Val (Val_Bits [BV{1} 1]) Mk_annot) Mk_annot
-     ] Mk_annot;
-        Ite (Binop Eq (Unop (SignExtend 64) (Val (Val_Symbolic 3444) Mk_annot) Mk_annot) (
-          Manyop (Bvmanyarith Bvadd) [
-            Manyop (Bvmanyarith Bvadd) [
-Unop (SignExtend 64) (Val (Val_Symbolic 3435) Mk_annot) Mk_annot;
-Val (Val_Bits [BV{128} 0xffffffffffffffffffffffffffffffff]) Mk_annot
-            ] Mk_annot;
-Val (Val_Bits [BV{128} 0x00000000000000000000000000000001]) Mk_annot
-          ] Mk_annot
-        ) Mk_annot)
-        (Val (Val_Bits [BV{1} 0]) Mk_annot) (Val (Val_Bits [BV{1} 1]) Mk_annot) Mk_annot
-   ] Mk_annot)) Mk_annot;
-  Smt (DefineConst 3459 (Unop (Extract 3 3) (Val (Val_Symbolic 3457) Mk_annot) Mk_annot)) Mk_annot;
-  ReadReg "PSTATE" [Field "N"] (Val_Struct [("N", (Val_Symbolic 29)) ]) Mk_annot;
-  WriteReg "PSTATE" [Field "N"] (Val_Struct [("N", (Val_Symbolic 3459)) ]) Mk_annot;
-  Smt (DefineConst 3460 (Unop (Extract 2 2) (Val (Val_Symbolic 3457) Mk_annot) Mk_annot)) Mk_annot;
-  ReadReg "PSTATE" [Field "Z"] (Val_Struct [ ("Z", (Val_Symbolic 15)) ]) Mk_annot;
-  WriteReg "PSTATE" [Field "Z"] (Val_Struct [ ("Z", (Val_Symbolic 3460)) ]) Mk_annot;
-  Smt (DefineConst 3461 (Unop (Extract 1 1) (Val (Val_Symbolic 3457) Mk_annot) Mk_annot)) Mk_annot;
-  ReadReg "PSTATE" [Field "C"] (Val_Struct [ ("C", (Val_Symbolic 20)) ]) Mk_annot;
-  WriteReg "PSTATE" [Field "C"] (Val_Struct [ ("C", (Val_Symbolic 3461)) ]) Mk_annot;
-  Smt (DefineConst 3462 (Unop (Extract 0 0) (Val (Val_Symbolic 3457) Mk_annot) Mk_annot)) Mk_annot;
-  ReadReg "PSTATE" [Field "V"] (Val_Struct [ ("V", (Val_Symbolic 25)) ]) Mk_annot;
-  WriteReg "PSTATE" [Field "V"] (Val_Struct [ ("V", (Val_Symbolic 3462)) ]) Mk_annot
-].
 
 (* trace of bne 0xc: (at address 0x0000000010300004)
   (* TODO: Can we somehoe merge the common parts of the two traces? *)
@@ -409,37 +222,6 @@ Definition trc_bne_0xc : list trc := [
 ]
 ].
 
-(* trace of b 0x8: (at 0x000000001030000c)
-  (read-reg |_PC| nil #x000000001030000c)
-  (branch-address #x0000000010300014)
-  (write-reg |_PC| nil #x0000000010300014)
-  (write-reg |__PC_changed| nil true))
-*)
-Definition trc_b_0x8 : trc := [
-  ReadReg "_PC" nil (Val_Bits [BV{64} 0x000000001030000c]) Mk_annot;
-  BranchAddress (Val_Bits [BV{64} 0x0000000010300014]) Mk_annot;
-  WriteReg "_PC" nil (Val_Bits [BV{64} 0x0000000010300014]) Mk_annot;
-  WriteReg "__PC_changed" nil (Val_Bool true) Mk_annot
-].
-
-(* trace of bl 0x100: (at address 0x0000000010300010)
-(trace
-  (read-reg |_PC| nil #x0000000010300010)
-  (write-reg |R30| nil #x0000000010300014)
-  (read-reg |_PC| nil #x0000000010300010)
-  (branch-address #x0000000010300110)
-  (write-reg |_PC| nil #x0000000010300110)
-  (write-reg |__PC_changed| nil true))
-*)
-Definition trc_bl_0x100' : trc := [
-  ReadReg "_PC" nil (Val_Bits [BV{64} 0x0000000010300010]) Mk_annot;
-  WriteReg "R30" nil (Val_Bits [BV{64} 0x0000000010300014]) Mk_annot;
-  ReadReg "_PC" nil (Val_Bits [BV{64} 0x0000000010300010]) Mk_annot;
-  BranchAddress (Val_Bits [BV{64} 0x0000000010300110]) Mk_annot;
-  WriteReg "_PC" nil (Val_Bits [BV{64} 0x0000000010300110]) Mk_annot;
-  WriteReg "__PC_changed" nil (Val_Bool true) Mk_annot
-].
-
 (*
 0x0000000010300000: cmp x1, 0
 0x0000000010300004: bne 0xc  --\
@@ -457,34 +239,22 @@ Definition test_state2_local (n1 : Z) Hin := {|
   seq_trace  := [];
   seq_regs   :=
     <[ "R1" := Val_Bits (BV 64 n1 Hin) ]> $
-    <[ "PSTATE" := (Val_Struct
-          [("GE", Val_Poison); ("F", Val_Bits [BV{1} 1]);
-          ("UAO", Val_Poison); ("C", Val_Bits [BV{1} 0]);
-          ("SP", Val_Poison); ("N", Val_Bits [BV{1} 0]);
-          ("Q", Val_Poison); ("A", Val_Bits [BV{1} 1]); ("SS", Val_Bits [BV{1} 0]);
-          ("E", Val_Poison); ("TCO", Val_Poison); ("I", Val_Bits [BV{1} 1]);
-          ("PAN", Val_Poison); ("M", Val_Poison); ("D", Val_Bits [BV{1} 1]);
-          ("nRW", Val_Bits [BV{1} 0]); ("EL", Val_Bits [BV{1} 0]);
-          ("IT", Val_Poison); ("IL", Val_Bits [BV{1} 0]);
-          ("Z", Val_Bits [BV{1} 0]); ("BTYPE", Val_Poison);
-          ("SSBS", Val_Poison); ("T", Val_Poison); ("J", Val_Poison);
-          ("V", Val_Bits [BV{1} 0]); ("DIT", Val_Bits [BV{1} 0])]) ]> $
     <[ "_PC" := Val_Bits start_address ]> $
     <[ "__PC_changed" := Val_Bool false ]> $
-                                             ∅;
+    sys_regs_map;
   seq_nb_state  := false;
 |}.
 Definition test_state2_global  := {|
   seq_instrs :=
-    <[[BV{64} 0x0000000010300000] := [trc_cmp_x1_0]]> $
+    <[[BV{64} 0x0000000010300000] := [cmp_x1_0_trace]]> $
     <[[BV{64} 0x0000000010300004] := trc_bne_0xc ]> $
-    <[[BV{64} 0x0000000010300008] := [trc_mov_x0_1]]> $
-    <[[BV{64} 0x000000001030000c] := [trc_b_0x8]]> $
-    <[[BV{64} 0x0000000010300010] := [trc_bl_0x100']]> $
-    <[[BV{64} 0x0000000010300014] := [trc_mov_OUT_x0]]> $
+    <[[BV{64} 0x0000000010300008] := [mov_x0_1_trace]]> $
+    <[[BV{64} 0x000000001030000c] := [b_0x8_trace]]> $
+    <[[BV{64} 0x0000000010300010] := [bl_0x100_trace]]> $
+    <[[BV{64} 0x0000000010300014] := [mov_x28_x0_trace]]> $
 
-    <[[BV{64} 0x0000000010300110] := [trc_mov_w0_0]]> $
-    <[[BV{64} 0x0000000010300114] := [trc_ret]]> $
+    <[[BV{64} 0x0000000010300110] := [mov_w0_0_trace]]> $
+    <[[BV{64} 0x0000000010300114] := [ret_trace]]> $
     ∅;
   seq_mem := ∅
 |}.
@@ -492,22 +262,23 @@ Definition test_state2_global  := {|
 Definition test_state2_spec : list seq_label := [ SInstrTrap [BV{64} 0x0000000010300018] ].
 
 Lemma test_state2_iris `{!islaG Σ} `{!threadG} n1 Hin :
-  instr 0x0000000010300000 (Some [trc_cmp_x1_0]) -∗
+  instr 0x0000000010300000 (Some [cmp_x1_0_trace]) -∗
   instr 0x0000000010300004 (Some trc_bne_0xc ) -∗
-  instr 0x0000000010300008 (Some [trc_mov_x0_1]) -∗
-  instr 0x000000001030000c (Some [trc_b_0x8]) -∗
-  instr 0x0000000010300010 (Some [trc_bl_0x100']) -∗
-  instr 0x0000000010300014 (Some [trc_mov_OUT_x0]) -∗
+  instr 0x0000000010300008 (Some [mov_x0_1_trace]) -∗
+  instr 0x000000001030000c (Some [b_0x8_trace]) -∗
+  instr 0x0000000010300010 (Some [bl_0x100_trace]) -∗
+  instr 0x0000000010300014 (Some [mov_x28_x0_trace]) -∗
   instr 0x0000000010300018 None -∗
-  instr 0x0000000010300110 (Some [trc_mov_w0_0]) -∗
-  instr 0x0000000010300114 (Some [trc_ret]) -∗
+  instr 0x0000000010300110 (Some [mov_w0_0_trace]) -∗
+  instr 0x0000000010300114 (Some [ret_trace]) -∗
 
+  reg_col sys_regs -∗
   "_PC" ↦ᵣ Val_Bits start_address -∗
   "__PC_changed" ↦ᵣ Val_Bool false -∗
   "R30" ↦ᵣ Val_Poison -∗
   "R1" ↦ᵣ Val_Bits (BV 64 n1 Hin) -∗
   "R0" ↦ᵣ Val_Poison -∗
-  "OUT" ↦ᵣ Val_Poison -∗
+  "R28" ↦ᵣ Val_Poison -∗
   "PSTATE" # "N" ↦ᵣ Val_Bits [BV{1} 0] -∗
   "PSTATE" # "Z" ↦ᵣ Val_Bits [BV{1} 0] -∗
   "PSTATE" # "C" ↦ᵣ Val_Bits [BV{1} 0] -∗
