instructions/branch.v
@@ -1,0 +1,36 @@
+From isla Require Import isla_lang.
+
+Definition branch_trace : trc := [
+  Smt (DeclareConst 28%Z (Ty_BitVec 1%N)) Mk_annot;
+(*  Cycle Mk_annot;*)
+(*  ReadReg "SEE" [] (Val_I (-1)%Z 128%Z) Mk_annot;*)
+(*  WriteReg "SEE" [] (Val_I 1215%Z 128%Z) Mk_annot;*)
+(*  WriteReg "__unconditional" [] (Val_Bool true) Mk_annot;*)
+(*  ReadReg "__v85_implemented" [] (Val_Bool false) Mk_annot;*)
+  Smt (DeclareConst 47%Z (Ty_BitVec 64%N)) Mk_annot;
+  ReadReg "_PC" [] (Val_Symbolic 47%Z) Mk_annot;
+  Smt (DefineConst 48%Z (Manyop (Bvmanyarith Bvadd) [Val (Val_Symbolic 47%Z) Mk_annot; Val (Val_Bits [BV{64%N} 0x10%Z]) Mk_annot] Mk_annot)) Mk_annot;
+  ReadReg "PSTATE" [Field "nRW"] (Val_Struct [("nRW", Val_Symbolic 28%Z)]) Mk_annot;
+  Smt (DefineConst 49%Z (Binop (Eq) (Val (Val_Symbolic 28%Z) Mk_annot) (Val (Val_Bits [BV{1%N} 0x1%Z]) Mk_annot) Mk_annot)) Mk_annot;
+  ReadReg "CFG_ID_AA64PFR0_EL1_EL0" [] (Val_Bits [BV{4%N} 0x1%Z]) Mk_annot;
+  ReadReg "CFG_ID_AA64PFR0_EL1_EL1" [] (Val_Bits [BV{4%N} 0x1%Z]) Mk_annot;
+  ReadReg "CFG_ID_AA64PFR0_EL1_EL2" [] (Val_Bits [BV{4%N} 0x1%Z]) Mk_annot;
+  ReadReg "CFG_ID_AA64PFR0_EL1_EL3" [] (Val_Bits [BV{4%N} 0x1%Z]) Mk_annot;
+  Smt (Assert (Unop (Not) (Val (Val_Symbolic 49%Z) Mk_annot) Mk_annot)) Mk_annot;
+(*  ReadReg "__highest_el_aarch32" [] (Val_Bool false) Mk_annot;*)
+  Smt (Assert (Unop (Not) (Val (Val_Symbolic 49%Z) Mk_annot) Mk_annot)) Mk_annot;
+  Smt (DefineConst 52%Z (Val (Val_Symbolic 48%Z) Mk_annot)) Mk_annot;
+  BranchAddress (Val_Symbolic 52%Z) Mk_annot;
+  Smt (DefineConst 53%Z (Val (Val_Symbolic 48%Z) Mk_annot)) Mk_annot;
+  Smt (DefineConst 54%Z (Binop (Eq) (Val (Val_Symbolic 28%Z) Mk_annot) (Val (Val_Bits [BV{1%N} 0x1%Z]) Mk_annot) Mk_annot)) Mk_annot;
+  Smt (Assert (Unop (Not) (Val (Val_Symbolic 54%Z) Mk_annot) Mk_annot)) Mk_annot;
+  Smt (Assert (Unop (Not) (Val (Val_Symbolic 54%Z) Mk_annot) Mk_annot)) Mk_annot;
+  ReadReg "PSTATE" [Field "EL"] (Val_Struct [("EL", Val_Bits [BV{2%N} 0x2%Z])]) Mk_annot;
+  ReadReg "SCR_EL3" [] (Val_Bits [BV{32%N} 0x0%Z]) Mk_annot;
+(*  ReadReg "__v81_implemented" [] (Val_Bool true) Mk_annot;*)
+(*  ReadReg "__v84_implemented" [] (Val_Bool false) Mk_annot;*)
+  ReadReg "TCR_EL2" [] (Val_Bits [BV{64%N} 0x0%Z]) Mk_annot;
+(*  ReadReg "__v83_implemented" [] (Val_Bool false) Mk_annot;*)
+  WriteReg "_PC" [] (Val_Symbolic 53%Z) Mk_annot;
+  WriteReg "__PC_changed" [] (Val_Bool true) Mk_annot
+].
