instructions/mov_x0_1.v
@@ -1,0 +1,10 @@
+From isla Require Import isla_lang.
+
+Definition mov_x0_1_trace : trc := [
+(*  Cycle Mk_annot;*)
+(*  ReadReg "SEE" [] (Val_I (-1)%Z 128%Z) Mk_annot;*)
+(*  WriteReg "SEE" [] (Val_I 1486%Z 128%Z) Mk_annot;*)
+(*  WriteReg "__unconditional" [] (Val_Bool true) Mk_annot;*)
+(*  ReadReg "__v85_implemented" [] (Val_Bool false) Mk_annot;*)
+  WriteReg "R0" [] (Val_Bits [BV{64%N} 0x1%Z]) Mk_annot
+].
